Finish the security Model & Refinement
Avoid using ugly record, use locale.function, quite neat now.

PiCore_IFS.thy
@@ -30,9 +30,6 @@ locale InfoFlow = event ptran petran fin_com
                                 dom_helper dome (gets P) (getx P) (Act (actk a)) (K (actk a)) = domain a}"*)
 begin
 
-definition noninterf :: "'d \<Rightarrow> 'd \<Rightarrow> bool" ("(_ \<setminus>\<leadsto> _)" [70,71] 60)
-  where "u \<setminus>\<leadsto> v \<equiv> \<not> (u \<leadsto> v)"
-
 definition vpeqC :: "('l,'k,'s, 'prog) pesconf \<Rightarrow> 'd \<Rightarrow> ('l,'k,'s, 'prog) pesconf \<Rightarrow> bool" ("(_ \<sim>._.\<sim> _)" [70,71] 60)
    where "vpeqC C1 u C2 \<equiv> (gets C1) \<sim>u\<sim> (gets C2)"
 
@@ -45,20 +42,15 @@ lemma vpeqC_symmetric: "\<forall> a b u. (a \<sim>.u.\<sim> b) \<longrightarrow>
 lemma vpeqC_reflexive: "\<forall> a u. (a \<sim>.u.\<sim> a)"
   by (simp add: vpeq_reflexive vpeqC_def)
 
-definition obsC :: " 'd \<Rightarrow> ('l,'k,'s,'prog) pesconf \<Rightarrow> 'o" (infixl "\<guillemotright>."  55)
-  where "obsC d C = (gets C) \<guillemotright> d"
+definition obsC :: " ('l,'k,'s,'prog) pesconf \<Rightarrow> 'd \<Rightarrow> 'o" (infixl "\<guillemotright>."  55)
+  where "C \<guillemotright>. d= (gets C) \<guillemotright> d"
 
-definition PiCore_SM :: "(('l,'k,'s,'prog) pesconf, 'd, ('l,'k,'s,'prog,'d) action, 'o) SM"
-  where "PiCore_SM \<equiv> \<lparr>s0 = C0, step = step, domain = domain, obs = obsC, vpeq = vpeqC, interference = interference\<rparr>"
-
-
-interpretation SM_IFS PiCore_SM 
-  by (smt (verit) PiCore_SM_def SM.select_convs(5) SM_IFS_def vpeqC_reflexive vpeqC_symmetric vpeqC_transitive)
+interpretation SM_IFS C0 step domain obsC vpeqC interference
+  using SM_IFS_def vpeqC_reflexive vpeqC_symmetric vpeqC_transitive by blast
 
 definition nextC :: "('l,'k,'s,'prog) pesconf \<Rightarrow> ('l,'k,'s,'prog,'d) action \<Rightarrow>  ('l,'k,'s,'prog) pesconf set" where
   "nextC P a \<equiv> {Q. (P,Q)\<in>step a}"
       
-
 primrec runC :: "('l,'k,'s,'prog,'d) action list \<Rightarrow> (('l,'k,'s,'prog) pesconf \<times> ('l,'k,'s,'prog) pesconf) set" where
   run_Nil:  "runC [] = Id " |
   run_Cons: "runC (a#as) = {(P,Q). (\<exists>R. (P,R) \<in> step a \<and> (R,Q) \<in> runC as)}"
@@ -69,15 +61,15 @@ definition reachablec :: "('l,'k,'s,'prog) pesconf \<Rightarrow> ('l,'k,'s,'prog
 definition reachablec0 :: "('l,'k,'s,'prog) pesconf \<Rightarrow> bool"  where
   "reachablec0 C \<equiv> reachablec C0 C"
 
-lemma run_equiv : "runC as = run PiCore_SM as"
+lemma run_equiv : "runC as = run as"
   apply (induct as, simp)
-  using PiCore_SM_def by auto
+  by (simp add: relcomp_unfold)
 
-lemma reachablec_equiv : "reachablec C1 C2 = reachable PiCore_SM C1 C2"
+lemma reachablec_equiv : "reachablec C1 C2 = reachable C1 C2"
   by (simp add: reachable_def reachablec_def run_equiv)
 
-lemma reachable0_equiv : "reachablec0 C = reachable0 PiCore_SM C"
-  by (simp add: PiCore_SM_def reachable0_def reachablec0_def reachablec_equiv)
+lemma reachable0_equiv : "reachablec0 C = reachable0  C"
+  by (simp add: reachable0_def reachablec0_def reachablec_equiv)
 
 subsection \<open>Unwinding Conditions\<close>
 
@@ -94,46 +86,46 @@ definition weak_step_consistentC :: "bool" where
                          \<and> ( ((domain a) \<leadsto> u) \<longrightarrow> (C1 \<sim>.(domain a).\<sim> C2) ) \<longrightarrow> 
                          (\<forall> C1' C2'. (C1'\<in>nextC C1 a) \<and> (C2'\<in>nextC C2 a) \<longrightarrow> (C1' \<sim>.u.\<sim> C2'))"
 
-lemma PiCore_obs_consistent : "observed_consistentC \<Longrightarrow> observed_consistent PiCore_SM"
-  by (simp add: PiCore_SM_def obsC_def observed_consistentC_def observed_consistent_def vpeqC_def)
+lemma PiCore_obs_consistent : "observed_consistentC \<Longrightarrow> observed_consistent "
+  by (simp add: obsC_def observed_consistentC_def observed_consistent_def vpeqC_def)
 
-lemma local_respectC_equiv : "local_respectC \<longleftrightarrow> local_respect PiCore_SM"
+lemma local_respectC_equiv : "local_respectC \<longleftrightarrow> local_respect"
 proof
   assume  "local_respectC"
-  then show "local_respect PiCore_SM"
+  then show "local_respect"
     apply (simp add: local_respectC_def local_respect_def, clarify)
     apply (drule_tac a = a and b = d and c = aa and d = ab and e = b in all5_imp2D)
       apply (simp add: reachable0_equiv)
-     apply (simp add: PiCore_SM_def noninterf_def)
-    by (simp add: PiCore_SM_def nextC_def)
+     apply (simp add:  noninterf_def)
+    by (simp add:  nextC_def)
 next
-  assume "local_respect PiCore_SM"
+  assume "local_respect"
   then show "local_respectC"
     apply (simp add: local_respectC_def local_respect_def, clarify)
     apply (drule_tac a = a and b = u and c = aa and d = ab and e = b in all5_impD)
     using reachable0_equiv apply auto[1]
-    by (simp add: PiCore_SM_def nextC_def noninterf_def)
+    by (simp add: nextC_def noninterf_def)
 qed
 
-lemma weak_step_consistentC_equiv : "weak_step_consistentC \<longleftrightarrow> weak_step_consistent PiCore_SM"
+lemma weak_step_consistentC_equiv : "weak_step_consistentC \<longleftrightarrow> weak_step_consistent"
 proof
   assume "weak_step_consistentC"
-  then show "weak_step_consistent PiCore_SM"
+  then show "weak_step_consistent"
     apply (simp add: weak_step_consistentC_def weak_step_consistent_def, clarify)
     apply (drule_tac a= a and b = d and c = aa and d = ab in all4D)
     apply (drule_tac a = b and b = ac and c = ad and d = ba in all4_imp2D)
     using reachable0_equiv apply presburger
-    using PiCore_SM_def apply force
-    by (simp add: PiCore_SM_def nextC_def)
+    apply force
+    by (simp add:  nextC_def)
 next
-  assume "weak_step_consistent PiCore_SM"
+  assume "weak_step_consistent "
   then show "weak_step_consistentC"
     apply (simp add: weak_step_consistentC_def weak_step_consistent_def, clarify)
     apply (drule_tac a= a and b = u and c = aa and d = ab in all4D)
     apply (drule_tac a = b and b = ac and c = ad and d = ba in all4_imp2D)
     using reachable0_equiv apply blast
-    using PiCore_SM_def apply force
-    using PiCore_SM_def nextC_def by force
+    apply force
+    using nextC_def by force
 qed
 
 
@@ -142,14 +134,14 @@ subsection \<open>Unwinding Theorem\<close>
 theorem PiCore_nonleakage:
     assumes p1: observed_consistentC
     and     p2: weak_step_consistentC 
-  shows "nonleakage PiCore_SM"
+  shows "nonleakage"
   using PiCore_obs_consistent UnwindingTheorem_nonleakage p1 p2 weak_step_consistentC_equiv by blast
 
 theorem PiCore_noninfluence0:
     assumes p1: observed_consistentC
     and     p2: local_respectC
     and     p3: weak_step_consistentC
-  shows "noninfluence0 PiCore_SM"
+  shows "noninfluence0"
   using PiCore_obs_consistent UnwindingTheorem_noninfluence0 local_respectC_equiv p1 p2 p3 weak_step_consistentC_equiv by fastforce
 
 end
