Refinement.thy
@@ -2,91 +2,118 @@ theory Refinement
   imports SecurityModel
 begin
 
-locale SM_Refine = SM_IFS mc + SM_IFS ma
-  for mc :: "('sc, 'd, 'ac, 'oc) SM"
-  and ma :: "('sa, 'd, 'aa, 'oa) SM" +
-fixes sim_s :: "'sc \<Rightarrow> 'sa" and
-      sim_a :: "'ac \<Rightarrow> 'aa option"
+locale SM_Refine = 
+  SM_IFS\<^sub>c: SM_IFS s0\<^sub>c step\<^sub>c domain\<^sub>c obs\<^sub>c vpeq\<^sub>c interference\<^sub>c +
+  SM_IFS\<^sub>a: SM_IFS s0\<^sub>a step\<^sub>a domain\<^sub>a obs\<^sub>a vpeq\<^sub>a interference\<^sub>a
+  for s0\<^sub>c :: "'s\<^sub>c"
+  and step\<^sub>c :: "'a\<^sub>c \<Rightarrow> ('s\<^sub>c \<times> 's\<^sub>c) set"
+  and domain\<^sub>c :: "'a\<^sub>c \<Rightarrow> 'd"
+  and obs\<^sub>c :: "'s\<^sub>c \<Rightarrow> 'd \<Rightarrow> 'o\<^sub>c" (infixl "\<guillemotright>\<^sub>c"  55)
+  and vpeq\<^sub>c :: "'s\<^sub>c \<Rightarrow> 'd \<Rightarrow> 's\<^sub>c \<Rightarrow> bool" ("(_ \<sim>\<^sub>c_\<sim>\<^sub>c _)" [70,69,70] 60)
+  and interference\<^sub>c :: "'d \<Rightarrow> 'd \<Rightarrow> bool" ("(_ \<leadsto>\<^sub>c _)" [70,71] 60)
+  and s0\<^sub>a :: "'s\<^sub>a"
+  and step\<^sub>a :: "'a\<^sub>a \<Rightarrow> ('s\<^sub>a \<times> 's\<^sub>a) set"
+  and domain\<^sub>a :: "'a\<^sub>a \<Rightarrow> 'd"
+  and obs\<^sub>a :: "'s\<^sub>a \<Rightarrow> 'd \<Rightarrow> 'o\<^sub>a" (infixl "\<guillemotright>\<^sub>a"  55)
+  and vpeq\<^sub>a :: "'s\<^sub>a \<Rightarrow> 'd \<Rightarrow> 's\<^sub>a \<Rightarrow> bool" ("(_ \<sim>\<^sub>a_\<sim>\<^sub>a _)" [70,69,70] 60)
+  and interference\<^sub>a :: "'d \<Rightarrow> 'd \<Rightarrow> bool" ("(_ \<leadsto>\<^sub>a _)" [70,71] 60) + 
+fixes sim_s :: "'s\<^sub>c \<Rightarrow> 's\<^sub>a"
+  and sim_a :: "'a\<^sub>c \<Rightarrow> 'a\<^sub>a option"
 assumes
-  init_sim : "sim_s (s0 mc) = s0 ma" and
-  action_refine : "sim_a ac = Some aa \<longrightarrow> (sc, tc) \<in> step mc ac \<longrightarrow> (sim_s sc, sim_s tc) \<in> step ma aa" and
-  none_refine : "sim_a ac = None \<longrightarrow> (sc, tc) \<in> step mc ac \<longrightarrow> sim_s sc = sim_s tc" and
-  intefere_same : "interference mc = interference ma" and 
-  dom_refine : "sim_a ac = Some aa \<longrightarrow> domain mc ac = domain ma aa" and 
-  sim_ifs : "vpeq ma (sim_s sc) d (sim_s tc) = vpeq mc sc d tc"    
-begin
+  init_sim : "sim_s s0\<^sub>c = s0\<^sub>a" and
+  action_refine : "sim_a a\<^sub>c = Some a\<^sub>a \<longrightarrow> (s\<^sub>c, t\<^sub>c) \<in> step\<^sub>c a\<^sub>c \<longrightarrow> (sim_s s\<^sub>c, sim_s t\<^sub>c) \<in> step\<^sub>a a\<^sub>a" and
+  none_refine : "sim_a a\<^sub>c = None \<longrightarrow> (s\<^sub>c, t\<^sub>c) \<in> step\<^sub>c a\<^sub>c \<longrightarrow> sim_s s\<^sub>c = sim_s t\<^sub>c" and
+  intefere_same : "interference\<^sub>c = interference\<^sub>a" and 
+  dom_refine : "sim_a a\<^sub>c = Some a\<^sub>a \<longrightarrow> domain\<^sub>c a\<^sub>c = domain\<^sub>a a\<^sub>a" and 
+  sim_ifs : "  (sim_s s\<^sub>c) \<sim>\<^sub>a d \<sim>\<^sub>a (sim_s t\<^sub>c) = s\<^sub>c \<sim>\<^sub>c d \<sim>\<^sub>c t\<^sub>c" 
+begin 
 
-lemma reachR_reach1: "\<forall>s as s'. reachable0 ma (sim_s s) \<and> reachable0 mc s \<and> s' \<in> execute mc as s
-                        \<longrightarrow> reachable0 ma (sim_s s')"
+abbreviation reachable0\<^sub>c :: "'s\<^sub>c \<Rightarrow> bool"
+  where "reachable0\<^sub>c \<equiv> SM_IFS\<^sub>c.reachable0"
+
+abbreviation reachable0\<^sub>a :: "'s\<^sub>a \<Rightarrow> bool"
+  where "reachable0\<^sub>a \<equiv> SM_IFS\<^sub>a.reachable0"
+
+abbreviation run\<^sub>c :: " 'a\<^sub>c list \<Rightarrow> ('s\<^sub>c \<times> 's\<^sub>c) set"
+  where "run\<^sub>c \<equiv> SM_IFS\<^sub>c.run"
+
+abbreviation execute\<^sub>c :: "'a\<^sub>c list \<Rightarrow> 's\<^sub>c \<Rightarrow> 's\<^sub>c set"
+  where "execute\<^sub>c \<equiv> SM_IFS\<^sub>c.execute"
+
+lemma reachR_reach1: "\<forall>s as s'. reachable0\<^sub>a (sim_s s) \<and> reachable0\<^sub>c s \<and> s' \<in> execute\<^sub>c as s
+                        \<longrightarrow> reachable0\<^sub>a  (sim_s s')"
 proof -
   {
     fix as
-    have "\<forall>s s'. reachable0 ma (sim_s s) \<and> reachable0 mc s \<and>  s' \<in> execute mc as s
-                        \<longrightarrow> reachable0 ma (sim_s s')"
+    have "\<forall>s s'. reachable0\<^sub>a (sim_s s) \<and> reachable0\<^sub>c s \<and> s' \<in> execute\<^sub>c as s \<longrightarrow> reachable0\<^sub>a (sim_s s')"
     proof(induct as)
-      case Nil show ?case by (simp add:execute_def)
+      case Nil show ?case 
+        by (simp add: SM_IFS\<^sub>c.execute_def)
     next
       case (Cons b bs)
-      assume a0: "\<forall>s s'. reachable0 ma (sim_s s) \<and> reachable0 mc s \<and> s' \<in> execute mc bs s 
-                   \<longrightarrow> reachable0 ma (sim_s s')"
+      assume a0: "\<forall>s s'. reachable0\<^sub>a (sim_s s) \<and> reachable0\<^sub>c s \<and> s' \<in> execute\<^sub>c bs s \<longrightarrow> reachable0\<^sub>a (sim_s s')"
       show ?case 
       proof -
         {
           fix s s'
-            assume b0: "reachable0 ma (sim_s s) \<and> reachable0 mc s \<and> s' \<in> execute mc (b # bs) s"
-            have b1: "\<forall>s1. (s, s1) \<in> (step mc) b \<longrightarrow> reachable0 ma (sim_s s1)"
-              by (metis action_refine b0 none_refine not_None_eq reachableStep)
-            from b0 have "\<exists>s1. (s,s1)\<in> (step mc) b \<and>  (s1 , s') \<in> run mc bs" using execute_def 
-              by (metis Image_singleton_iff relcompEpair run_Cons)
-            then obtain s1 where b2: "(s,s1) \<in> (step mc) b \<and>  (s1 , s') \<in> run mc bs" by auto
-            with b1 have b3: "reachable0 ma (sim_s s1)" by simp
-            have b4: "reachable0 mc s1" by (meson b0 b2 reachableStep) 
-            with a0 b2 b3 have "reachable0 ma (sim_s s')" 
-              by (metis Image_singleton_iff execute_def)
-          }
-          then show ?thesis by auto
-        qed
+          assume b0: "reachable0\<^sub>a (sim_s s) \<and> reachable0\<^sub>c  s \<and> s' \<in> execute\<^sub>c (b # bs) s"
+          have b1: "\<forall>s1. (s, s1) \<in> step\<^sub>c b \<longrightarrow> reachable0\<^sub>a (sim_s s1)"
+            by (metis SM_IFS\<^sub>a.reachableStep action_refine b0 none_refine option.exhaust)
+          from b0 have "\<exists>s1. (s,s1)\<in> step\<^sub>c b \<and>  (s1 , s') \<in> run\<^sub>c bs"   
+            using SM_IFS\<^sub>c.execute_def by auto
+          then obtain s1 where b2: "(s,s1)\<in> step\<^sub>c b \<and>  (s1 , s') \<in> run\<^sub>c bs" by auto
+          with b1 have b3: "reachable0\<^sub>a (sim_s s1)" by simp
+          have b4: "reachable0\<^sub>c s1" 
+            using SM_IFS\<^sub>c.reachableStep b0 b2 by blast
+          with a0 b2 b3 have "reachable0\<^sub>a (sim_s s')"
+            by (metis Image_singleton_iff SM_IFS.execute_def SM_IFS\<^sub>c.SM_IFS_axioms)
+        }
+        then show ?thesis by auto
       qed
-    }
-    then show ?thesis by auto
-  qed
+    qed
+  }
+  then show ?thesis by auto
+qed
 
+lemma reachR_reach: "reachable0\<^sub>c sc \<Longrightarrow> reachable0\<^sub>a (sim_s sc)"
+  by (metis Image_singleton_iff SM_IFS.execute_def SM_IFS\<^sub>a.reachableC0 SM_IFS\<^sub>c.SM_IFS_axioms 
+     SM_IFS\<^sub>c.reachable0_def SM_IFS\<^sub>c.reachableC0 SM_IFS\<^sub>c.reachable_def init_sim reachR_reach1)
 
-lemma reachR_reach: "reachable0 mc sc \<Longrightarrow> reachable0 ma (sim_s sc)"
-  by (metis Image_singleton_iff execute_def init_sim reachR_reach1 reachable0_def reachable_def reachable_s0)
+thm SM_IFS\<^sub>a.local_respect_def
 
-theorem abs_lr_imp : "local_respect ma \<Longrightarrow> local_respect mc"
+theorem abs_lr_imp : "SM_IFS\<^sub>a.local_respect \<Longrightarrow> SM_IFS\<^sub>c.local_respect"
 proof-
-  assume a0: "local_respect ma"
-  then have a1: "\<forall>aa d sa sa'. reachable0 ma sa \<longrightarrow> (\<not> interference ma (domain ma aa) d) 
-                 \<and> (sa, sa') \<in> (step ma) aa \<longrightarrow> (vpeq ma sa d sa')"
-    by (simp add: local_respect_def)
-  have "\<forall>ac d sc sc'. reachable0 mc sc \<longrightarrow> (\<not> interference mc (domain mc ac) d) 
-                          \<and> (sc, sc') \<in> step mc ac \<longrightarrow> (vpeq mc sc d sc')"
+  assume a0: "SM_IFS\<^sub>a.local_respect"
+  then have a1: "\<forall>aa d sa sa'. reachable0\<^sub>a sa \<longrightarrow> \<not> domain\<^sub>a aa \<leadsto>\<^sub>a d 
+                 \<and> (sa, sa') \<in> step\<^sub>a aa \<longrightarrow> (sa \<sim>\<^sub>a d \<sim>\<^sub>a sa')"
+    by (simp add: SM_IFS\<^sub>a.local_respect_def)
+  have "\<forall>ac d sc sc'. reachable0\<^sub>c sc \<longrightarrow> \<not> domain\<^sub>c ac \<leadsto>\<^sub>a d \<and> (sc, sc') \<in> step\<^sub>c ac 
+                      \<longrightarrow> (sc \<sim>\<^sub>c d \<sim>\<^sub>c sc')"
   proof-
     {
       fix ac d sc sc'
-      assume b0: "reachable0 mc sc"
-        and  b1: "\<not> interference mc (domain mc ac) d"
-        and  b2: "(sc, sc') \<in> step mc ac"
-      have "vpeq mc sc d sc'"
+      assume b0: "reachable0\<^sub>c sc"
+        and  b1: "\<not> domain\<^sub>c ac \<leadsto>\<^sub>a d"
+        and  b2: "(sc, sc') \<in> step\<^sub>c ac "
+      have "sc \<sim>\<^sub>c d \<sim>\<^sub>c sc'"
       proof(cases "sim_a ac = None")
         assume c0: "sim_a ac = None"
         with b2 have "sim_s sc = sim_s sc'" by (meson none_refine)
         then show ?thesis
-          by (metis sim_ifs vpeq_reflexive_lemma)
+          by (metis SM_IFS\<^sub>c.vpeq_reflexive sim_ifs)
       next
         assume d0: "\<not> sim_a ac = None"
         then have  "\<exists>aa. sim_a ac = Some aa" by auto
         then obtain aa where d1: "sim_a ac = Some aa" by force
-        then have  "domain mc ac = domain ma aa"
+        then have d01: "domain\<^sub>c ac = domain\<^sub>a aa"
           by (simp add: dom_refine)
-        with b1 have d2 :"\<not> interference ma (domain ma aa) d"
+        with b1 have d2 :"\<not> domain\<^sub>c ac \<leadsto>\<^sub>a d"
           by (simp add: intefere_same)
-        from b0 have d3: "reachable0 ma (sim_s sc)" by (simp add: reachR_reach)
-        from b2 have d4: "(sim_s sc, sim_s sc') \<in> step ma aa"
+        from b0 have d3: "reachable0\<^sub>a (sim_s sc)" by (simp add: reachR_reach)
+        from b2 have d4: "(sim_s sc, sim_s sc') \<in> step\<^sub>a aa"
           using action_refine d1 by blast
-        with a1 d2 d3 have "vpeq ma (sim_s sc) d (sim_s sc')" by blast
+        with a1 d2 d3 have "sim_s sc \<sim>\<^sub>a d \<sim>\<^sub>a sim_s sc'"
+          by (simp add: d01)
         then show ?thesis 
           using sim_ifs by blast
       qed
@@ -94,33 +121,35 @@ proof-
     then show ?thesis by auto
   qed
   then show ?thesis 
-    by (simp add: local_respect_def)
+    using SM_IFS\<^sub>c.local_respect_def intefere_same by blast
 qed
 
-theorem abs_wsc_imp : "weak_step_consistent ma \<Longrightarrow> weak_step_consistent mc"
+thm SM_IFS\<^sub>a.weak_step_consistent_def
+
+theorem abs_wsc_imp : "SM_IFS\<^sub>a.weak_step_consistent \<Longrightarrow> SM_IFS\<^sub>c.weak_step_consistent"
 proof-
-  assume a0: "weak_step_consistent ma"
-  then have a1: "\<forall>aa d sa ta. reachable0 ma sa \<and> reachable0 ma ta \<longrightarrow> (vpeq ma sa d ta) \<and> 
-                 ((interference ma (domain ma aa) d) \<longrightarrow> (vpeq ma sa (domain ma  aa) ta)) 
-                 \<longrightarrow> (\<forall> sa' ta'. (sa,sa') \<in> step ma aa \<and> (ta,ta') \<in> step ma aa \<longrightarrow> vpeq ma sa' d ta')"
-    by (smt (verit, ccfv_SIG) weak_step_consistent_def)
-  have "\<forall>ac d sc tc. reachable0 mc sc \<and> reachable0 mc tc \<longrightarrow> (vpeq mc sc d tc) \<and> 
-         ((interference mc (domain mc ac) d) \<longrightarrow> (vpeq mc sc (domain mc ac) tc)) 
-         \<longrightarrow> (\<forall> sc' tc'. (sc,sc') \<in> step mc ac \<and> (tc,tc') \<in> step mc ac \<longrightarrow> vpeq mc sc' d tc')"
+  assume a0: "SM_IFS\<^sub>a.weak_step_consistent"
+  then have a1: "\<forall>aa d sa ta. reachable0\<^sub>a sa \<and> reachable0\<^sub>a ta \<longrightarrow> (sa \<sim>\<^sub>a d \<sim>\<^sub>a ta) \<and> 
+                 (domain\<^sub>a aa \<leadsto>\<^sub>a d \<longrightarrow> sa \<sim>\<^sub>a domain\<^sub>a aa \<sim>\<^sub>a ta) 
+                 \<longrightarrow> (\<forall>sa' ta'. (sa, sa') \<in> step\<^sub>a aa \<and> (ta, ta') \<in> step\<^sub>a aa \<longrightarrow> sa' \<sim>\<^sub>a d \<sim>\<^sub>a ta')"
+    using SM_IFS\<^sub>a.weak_step_consistent_def by blast
+  have "\<forall>ac d sc tc. reachable0\<^sub>c sc \<and> reachable0\<^sub>c tc \<longrightarrow> (sc \<sim>\<^sub>c d \<sim>\<^sub>c tc) \<and> 
+                 (domain\<^sub>c ac \<leadsto>\<^sub>c d \<longrightarrow> sc \<sim>\<^sub>c domain\<^sub>c ac \<sim>\<^sub>c tc) 
+                 \<longrightarrow> (\<forall>sc' tc'. (sc, sc') \<in> step\<^sub>c ac \<and> (tc, tc') \<in> step\<^sub>c ac \<longrightarrow> sc' \<sim>\<^sub>c d \<sim>\<^sub>c tc')"
   proof-
     {
       fix ac d sc tc
-      assume b0: "reachable0 mc sc"
-        and  b1: "reachable0 mc tc"
-        and  b2: "vpeq mc sc d tc"
-        and  b3: "(interference mc (domain mc ac) d) \<longrightarrow> (vpeq mc sc (domain mc ac) tc)"
-      have "\<forall>sc' tc'. (sc,sc') \<in> step mc ac \<and> (tc,tc') \<in> step mc ac \<longrightarrow> vpeq mc sc' d tc'"
+      assume b0: "reachable0\<^sub>c sc"
+        and  b1: "reachable0\<^sub>c tc"
+        and  b2: "sc \<sim>\<^sub>c d \<sim>\<^sub>c tc"
+        and  b3: "domain\<^sub>c ac \<leadsto>\<^sub>c d \<longrightarrow> sc \<sim>\<^sub>c domain\<^sub>c ac \<sim>\<^sub>c tc"
+      have "\<forall>sc' tc'. (sc, sc') \<in> step\<^sub>c ac \<and> (tc, tc') \<in> step\<^sub>c ac \<longrightarrow> sc' \<sim>\<^sub>c d \<sim>\<^sub>c tc'"
       proof-
         {
           fix sc' tc'
-          assume c0: "(sc,sc') \<in> step mc ac"
-            and  c1: "(tc,tc') \<in> step mc ac"
-          have "vpeq mc sc' d tc'"
+          assume c0: "(sc,sc') \<in> step\<^sub>c ac"
+            and  c1: "(tc,tc') \<in> step\<^sub>c ac"
+          have "sc' \<sim>\<^sub>c d \<sim>\<^sub>c tc'"
           proof(cases "sim_a ac = None")
             assume "sim_a ac = None"
             then have "sim_s sc' = sim_s sc \<and> sim_s tc' = sim_s tc"
@@ -130,26 +159,23 @@ proof-
             assume "\<not> sim_a ac = None"
             then have "\<exists>aa. sim_a ac = Some aa" by auto
             then obtain aa where d0: "sim_a ac = Some aa" by auto
-            from b0 have d1: "reachable0 ma (sim_s sc)"
+            from b0 have d1: "reachable0\<^sub>a (sim_s sc)"
               by (simp add: reachR_reach)
-            from b1 have d2: "reachable0 ma (sim_s tc)"
+            from b1 have d2: "reachable0\<^sub>a (sim_s tc)"
               by (simp add: reachR_reach)
-            from b2 have d3: "vpeq ma (sim_s sc) d (sim_s tc)"
+            from b2 have d3: "sim_s sc \<sim>\<^sub>a d \<sim>\<^sub>a sim_s tc"
               using sim_ifs by blast
-          from d0 have d5 : "domain mc ac = domain ma  aa"
+          from d0 have d5 : "domain\<^sub>c ac = domain\<^sub>a aa"
             using dom_refine by blast
-          then have d6: "interference mc (domain mc ac) d = 
-                         interference ma (domain ma aa) d"
+          then have d6: " domain\<^sub>c ac \<leadsto>\<^sub>c d =  domain\<^sub>a aa \<leadsto>\<^sub>c d"
             by (simp add: intefere_same)
-          from d5 have d7 : "vpeq mc sc (domain mc ac) tc = 
-                             vpeq ma (sim_s sc) (domain ma aa) (sim_s tc)"
+          from d5 have d7 : "sc \<sim>\<^sub>c domain\<^sub>c ac \<sim>\<^sub>c tc = sim_s sc \<sim>\<^sub>a domain\<^sub>a aa \<sim>\<^sub>a sim_s tc"
             using sim_ifs by auto
-          with b3 d6 have d8: "(interference ma (domain ma aa) d) 
-                \<longrightarrow> (vpeq ma (sim_s sc) (domain ma aa) (sim_s tc))"
-            by blast
-          from c0 c1 have "(sim_s sc, sim_s sc') \<in> step ma aa \<and> (sim_s tc, sim_s tc') \<in> step ma aa"
+          with b3 d6 have d8: " domain\<^sub>a aa \<leadsto>\<^sub>a d \<longrightarrow> sim_s sc \<sim>\<^sub>a domain\<^sub>a aa \<sim>\<^sub>a sim_s tc"
+            using intefere_same by fastforce
+          from c0 c1 have "(sim_s sc, sim_s sc') \<in> step\<^sub>a aa \<and> (sim_s tc, sim_s tc') \<in> step\<^sub>a aa"
             using action_refine d0 by blast
-          with a1 d1 d2 d3 d8 have "vpeq ma (sim_s sc') d (sim_s tc')"  by blast
+          with a1 d1 d2 d3 d8 have "sim_s sc' \<sim>\<^sub>ad\<sim>\<^sub>a sim_s tc'"  by blast
           then show ?thesis
             using sim_ifs by blast
         qed
@@ -160,14 +186,11 @@ proof-
     then show ?thesis by blast
   qed
   then show ?thesis
-    using weak_step_consistent_def by blast
+    using SM_IFS\<^sub>c.weak_step_consistent_def by fastforce
 qed
-  
+
 
 end
-  
-
-
 
 
 end
