SecurityModel.thy
@@ -4,70 +4,54 @@ begin
 
 subsection \<open> Security State Machine \<close>
 
+locale SM_IFS = 
+  fixes s0  :: "'s"
+  and step :: "'a \<Rightarrow> ('s \<times> 's) set"
+  and domain :: "'a \<Rightarrow> 'd"
+  and obs :: "'s \<Rightarrow> 'd \<Rightarrow> 'o" (infixl "\<guillemotright>"  55)
+  and vpeq :: "'s \<Rightarrow> 'd \<Rightarrow> 's \<Rightarrow> bool" ("(_ \<sim>_\<sim> _)" [70,69,70] 60)
+  and interference :: "'d \<Rightarrow> 'd \<Rightarrow> bool" ("(_ \<leadsto> _)" [70,71] 60)
+assumes vpeq_transitive : "\<forall> a b c u. (a \<sim> u \<sim> b) \<and> (b \<sim> u \<sim> c) \<longrightarrow> (a \<sim> u \<sim> c)"
+    and vpeq_symmetric : "\<forall> a b u. (a \<sim> u \<sim> b) \<longrightarrow> (b \<sim> u \<sim> a)"
+    and vpeq_reflexive : "\<forall> a u. (a \<sim> u \<sim> a)"
+begin
 
-record ('s, 'd, 'a, 'o) SM = 
-  s0 :: "'s"
-  step :: "'a \<Rightarrow> ('s \<times> 's) set"
-  domain :: "'a \<Rightarrow> 'd"
-  obs :: "'d \<Rightarrow> 's \<Rightarrow> 'o"
-  vpeq :: "'s \<Rightarrow> 'd \<Rightarrow> 's \<Rightarrow> bool" 
-  interference :: "'d \<Rightarrow> 'd \<Rightarrow> bool" 
+definition noninterf :: "'d \<Rightarrow> 'd \<Rightarrow> bool" ("(_ \<setminus>\<leadsto> _)" [70,71] 60)
+  where "u \<setminus>\<leadsto> v \<equiv> \<not> (u \<leadsto> v)"
 
-primrec run :: "('s, 'd, 'a, 'o) SM \<Rightarrow> 'a list \<Rightarrow> ('s \<times> 's) set" 
-  where run_Nil: "run m [] = Id" |
-  run_Cons: "run m (a#as) = (step m) a O run m as"
 
-definition ivpeq :: "('s, 'd, 'a, 'o) SM \<Rightarrow> 's \<Rightarrow> 'd set \<Rightarrow> 's \<Rightarrow> bool" 
-  where "ivpeq m s D t \<equiv> \<forall> d \<in> D. vpeq m s d t"
+definition ivpeq :: "'s \<Rightarrow> 'd set \<Rightarrow> 's \<Rightarrow> bool" ("(_ \<approx> _ \<approx> _)" [70,71] 60)
+  where "ivpeq s D t \<equiv> \<forall> d \<in> D. (s \<sim> d \<sim> t)"
 
-definition next_states :: "('s, 'd, 'a, 'o) SM \<Rightarrow> 's \<Rightarrow> 'a \<Rightarrow> 's set"
-  where "next_states m s a \<equiv> {Q. (s,Q)\<in> step m a}"
+primrec run :: " 'a list \<Rightarrow> ('s \<times> 's) set" 
+  where run_Nil: "run  [] = Id" |
+  run_Cons: "run (a#as) = step a O run as"
 
-definition execute  :: "('s, 'd, 'a, 'o) SM \<Rightarrow> 'a list \<Rightarrow> 's \<Rightarrow> 's set" 
-  where "execute m as s = Image (run m as) {s} " 
+definition execute  :: " 'a list \<Rightarrow> 's \<Rightarrow> 's set" 
+  where "execute as s = Image (run as) {s}"
 
-definition reachable :: " ('s, 'd, 'a, 'o) SM \<Rightarrow> 's \<Rightarrow> 's \<Rightarrow> bool"
-  where "reachable m s1 s2 \<equiv>  (\<exists>as. (s1,s2) \<in> run m as)"
-
-definition reachable0 :: "('s, 'd, 'a, 'o) SM \<Rightarrow> 's \<Rightarrow> bool" 
-  where "reachable0 m s \<equiv> reachable m (s0 m)  s"
-
-lemma reachable_s0 : "reachable0 m (s0 m) "
-  by (metis pair_in_Id_conv reachable0_def reachable_def run_Nil)
-
-lemma reachable_self : "reachable m s s"
-  by (metis pair_in_Id_conv reachable_def run_Nil)
-
-lemma reachable_step : " (s , s') \<in> step m a \<Longrightarrow> reachable m s s'"
+lemma run_trans : "\<forall>s t v as bs. (C,T)\<in>run as \<and> (T,V)\<in>run bs \<longrightarrow> (C,V)\<in>run (as@bs)"
 proof-
-  assume a0: "(s , s') \<in> step m a"
-  then have "(s,s') \<in> run m [a]" by simp
-  then show ?thesis 
-    by (meson reachable_def)
-qed
-
-
-lemma run_trans : "\<forall>C T V as bs. (C,T)\<in> run m as \<and> (T,V) \<in> run m bs \<longrightarrow> (C,V) \<in> run m (as@bs)"
-proof -
   {
     fix T V as bs
-    have "\<forall>C. (C,T)\<in> run m as \<and> (T,V) \<in> run m bs \<longrightarrow> (C,V) \<in> run m (as@bs)"
+    have "\<forall>C. (C,T)\<in>run as \<and> (T,V)\<in>run bs \<longrightarrow> (C,V)\<in>run (as@bs)"
     proof(induct as)
       case Nil show ?case by simp
     next
       case (Cons c cs)
-      assume a0: "\<forall>C. (C, T) \<in> run m cs \<and> (T, V) \<in> run m bs \<longrightarrow> (C, V) \<in> run m (cs @ bs)"
+      assume a0: "\<forall>C. (C, T) \<in> run cs \<and> (T, V) \<in> run bs \<longrightarrow> (C, V) \<in> run (cs @ bs)"
       show ?case
       proof-
         {
           fix C
-          have "(C, T) \<in> run m (c # cs) \<and> (T, V) \<in> run m bs \<longrightarrow> (C, V) \<in> run m ((c # cs) @ bs) "
+          have "(C, T) \<in> run (c # cs) \<and> (T, V) \<in> run bs \<longrightarrow> (C, V) \<in> run ((c # cs) @ bs) "
           proof
-            assume b0: "(C, T) \<in> run m (c # cs) \<and> (T, V) \<in> run m bs"
-            from b0 obtain C' where b2: "(C,C')\<in> step m c \<and> (C',T)\<in> run m cs" by auto
-            with a0 b0 have "(C',V)\<in>run m (cs@bs)" by blast
-            with b2 show "(C, V) \<in> run m ((c # cs) @ bs)"
-              using append_Cons relcomp.relcompI run_Cons by auto 
+            assume b0: "(C, T) \<in> run (c # cs) \<and> (T, V) \<in> run bs"
+                (*assume b1: "(T, V) \<in> run bs"*)
+            from b0 obtain C' where b2: "(C,C')\<in>step c \<and> (C',T)\<in>run cs" by auto
+            with a0 b0 have "(C',V)\<in>run (cs@bs)" by blast
+            with b2 show "(C, V) \<in> run ((c # cs) @ bs)"
+              by auto
           qed
         }
         then show ?thesis by auto
@@ -77,107 +61,207 @@ proof -
   then show ?thesis by auto
 qed
 
+definition reachable :: "'s \<Rightarrow> 's \<Rightarrow> bool" ("(_ \<hookrightarrow> _)" [70,71] 60) where
+  "reachable s t \<equiv>  (\<exists>as. (s, t) \<in> run as)"
 
-lemma reachable_trans : "\<lbrakk>reachable m C T; reachable m T V\<rbrakk> \<Longrightarrow> reachable m C V"
+definition reachable0 :: "'s \<Rightarrow> bool"  where
+  "reachable0 s \<equiv> reachable s0 s"
+
+lemma reachableC0 : "reachable0 s0"
+  by (metis IdI reachable0_def reachable_def run_Nil)
+
+lemma reachable_self : "reachable s s"
+  by (metis IdI reachable_def run_Nil)
+  
+lemma reachable_step : "(s, s')\<in>step a \<Longrightarrow> reachable s s'"
 proof-
-  assume a0: "reachable m C T"
-  assume a1: "reachable m T V"
-  from a0 have "C = T \<or> (\<exists>as. (C,T)\<in>run m as)" using reachable_def 
+  assume a0: "(s, s')\<in>step a"
+  then have "(s , s')\<in>run [a]"
+    by simp
+  then show ?thesis
+    using reachable_def by blast
+qed
+
+lemma reachable_trans : "\<lbrakk>reachable C T; reachable T V\<rbrakk> \<Longrightarrow> reachable C V"
+proof-
+  assume a0: "reachable C T"
+  assume a1: "reachable T V"
+  from a0 have "C = T \<or> (\<exists>as. (C,T)\<in>run as)" using reachable_def 
     by metis
   then show ?thesis
   proof
     assume b0: "C = T"
     show ?thesis 
     proof -
-      from a1 have "T = V \<or> (\<exists>as. (T,V)\<in>run m as)" using reachable_def by metis
+      from a1 have "T = V \<or> (\<exists>as. (T,V)\<in>run  as)" using reachable_def by metis
       then show ?thesis
       proof
         assume c0: "T=V"
         with a0 show ?thesis by simp
       next
-        assume c0: "(\<exists>as. (T,V)\<in>run m as)"
+        assume c0: "(\<exists>as. (T,V)\<in>run  as)"
         then show ?thesis by (simp add: a1 b0) 
       qed
     qed
   next
-    assume b0: "\<exists>as. (C,T)\<in>run m as"
+    assume b0: "\<exists>as. (C,T)\<in>run as"
     show ?thesis
     proof -
-      from a1 have "T = V \<or> (\<exists>as. (T,V)\<in>run m as)" using reachable_def by metis
+      from a1 have "T = V \<or> (\<exists>as. (T,V)\<in>run  as)" using reachable_def by metis
       then show ?thesis
       proof
         assume c0: "T=V"
         then show ?thesis using a0 by auto 
       next
-        assume c0: "(\<exists>as. (T,V)\<in>run m as)"
-        from b0 obtain as where d0: "(C,T)\<in>run m as" by auto
-        from c0 obtain bs where d1: "(T,V)\<in>run m bs" by auto
+        assume c0: "(\<exists>as. (T,V)\<in>run  as)"
+        from b0 obtain as where d0: "(C,T)\<in>run as" by auto
+        from c0 obtain bs where d1: "(T,V)\<in>run bs" by auto
         then show ?thesis using d0 reachable_def run_trans by metis 
       qed
     qed
   qed
 qed
 
-lemma reachableStep : "\<lbrakk>reachable0 m C; (C,C')\<in> step m a\<rbrakk> \<Longrightarrow> reachable0 m C'"
-proof -
-  assume a0: "reachable0 m C"
-  assume a1: "(C,C')\<in>(step m) a"
-  from a0 have "(C = (s0 m)) \<or> (\<exists>as. ((s0 m),C) \<in> run m as)" unfolding reachable0_def reachable_def by auto
-  then show "reachable0 m C'"
-  proof
-    assume b0: "C = s0 m"
-    show "reachable0 m C'"
-      using a1 b0 reachable0_def reachable_step by metis
-  next
-    assume b0: "\<exists>as. ((s0 m),C) \<in> run m as"
-    show "reachable0 m C'"
-      using a0 a1 reachable0_def reachable_step reachable_trans by metis 
+lemma reachableStep : "\<lbrakk>reachable0 C; (C,C')\<in>step a\<rbrakk> \<Longrightarrow> reachable0 C'"
+  proof -
+    assume a0: "reachable0 C"
+    assume a1: "(C,C')\<in>step a"
+    from a0 have "(C = s0) \<or> (\<exists>as. (s0,C) \<in> run as)" unfolding reachable0_def reachable_def by auto
+    then show "reachable0 C'"
+      proof
+        assume b0: "C = s0"
+        show "reachable0 C'"
+          using a1 b0 reachable0_def reachable_step by auto 
+      next
+        assume b0: "\<exists>as. (s0,C) \<in> run as"
+        show "reachable0 C'"
+          using a0 a1 reachable0_def reachable_step reachable_trans by blast 
+      qed
   qed
-qed
-    
-lemma reachable0_reach : "\<lbrakk>reachable0 m C; reachable m C C'\<rbrakk> \<Longrightarrow> reachable0 m C'"
-  using reachable0_def reachable_trans by metis
 
-primrec sources :: "('s, 'd, 'a, 'o) SM \<Rightarrow> 'a list  \<Rightarrow> 'd \<Rightarrow> 'd set"
-  where sources_Nil:"sources m [] d = {d}" |
-  sources_Cons: "sources m (a # as) d = (sources m as d) \<union> {w. w = (domain m) a \<and> 
-                                        (\<exists>v. interference m w v \<and> v \<in> sources m as d) }"
-
-declare sources_Nil [simp del]   
+lemma reachable0_reach : "\<lbrakk>reachable0 C; reachable C C'\<rbrakk> \<Longrightarrow> reachable0 C'"
+  using reachable0_def reachable_trans by blast
+  
+primrec sources :: "'a list \<Rightarrow> 'd \<Rightarrow> 'd set" where
+  sources_Nil:  "sources [] u = {u}" |
+  sources_Cons: "sources (a#as) u = (sources as u) \<union> {w. w = domain a \<and> (\<exists>v. (w \<leadsto> v) \<and> v \<in> sources as u)}"
+declare sources_Nil [simp del]    
 declare sources_Cons [simp del]
 
+primrec ipurge :: "'a list \<Rightarrow> 'd \<Rightarrow> 'a list" where
+  ipurge_Nil:   "ipurge [] u = []" |
+  ipurge_Cons:  "ipurge (a#as) u = (if  domain a \<in> sources (a#as) u then
+                                          a # ipurge as u
+                                       else
+                                          ipurge as u
+                                      )"
 
-primrec ipurge :: "('s, 'd, 'a, 'o) SM  \<Rightarrow> 'a list \<Rightarrow> 'd \<Rightarrow> 'a list"
-  where ipurge_Nil:   "ipurge m [] u  = []" |
-  ipurge_Cons:  "ipurge m (a#as) u = (if (domain m) a \<in> (sources m (a#as) u) then
-                                              a # ipurge m as u 
-                                           else
-                                              ipurge m as u 
-                                          )"
+lemma sources_ipurge: "sources (ipurge as u) u = sources as u"
+  proof -
+    have "\<forall>as u. sources (ipurge as u) u = sources as u"
+    proof -
+      {
+        fix as
+        have "\<forall>u. sources (ipurge as u) u = sources as u"
+          proof(induct as)
+            case Nil show ?case by simp
+          next
+            case (Cons b bs)
+            assume a0: "\<forall>u. sources (ipurge bs u) u = sources bs u"
+            show ?case
+            proof -
+            {
+              fix u
+              have "sources (ipurge (b # bs) u) u = sources (b # bs) u"
+                proof(cases "domain b\<in>sources (b#bs) u")
+                  assume b0: "domain b\<in>sources (b#bs) u"
+                  then have b1: "ipurge (b # bs) u = b # ipurge bs u"
+                    by (simp add: sources_Cons) 
+                  from a0 have b2: "sources (ipurge bs u) u = sources bs u" by simp
+                  from b1 have b3: "sources (ipurge (b # bs) u) u = sources (b # ipurge bs u) u" by simp
+                  with b0 b2 have b4: "sources (ipurge (b # bs) u) u = {domain b} \<union> sources (ipurge bs u) u"
+                    using sources_Cons by auto
+                  from b0 have b5: "sources (b # bs) u = {domain b} \<union> sources bs u" using sources_Cons by auto 
+                  then show ?thesis using a0 b4 by auto 
+                next
+                  assume b0: "\<not> domain b\<in>sources (b#bs) u"
+                  then have b1: "sources (ipurge (b # bs) u) u = sources (ipurge bs u) u" using sources_Cons by auto 
+                  from b0 have b2: "sources (b # bs) u = sources bs u" using sources_Cons by auto 
+                  with a0 b1 show ?thesis by auto
+                qed
+            }
+            then show ?thesis by auto
+            qed
+        qed
+      }
+      then show ?thesis by auto
+      qed
+    then show ?thesis by auto
+    qed
 
-definition exec_equiv :: "('s, 'd, 'a, 'o) SM \<Rightarrow> 's \<Rightarrow> 'a list \<Rightarrow> 's \<Rightarrow> 'a list \<Rightarrow> 'd \<Rightarrow> bool" 
-  where "exec_equiv m s as t bs d \<equiv>  \<forall>s' t'. ((s,s')\<in> run m as \<and> (t,t')\<in> run m bs) 
-        \<longrightarrow> obs m d s' = obs m d t'"
+lemma ipurge_eq: "ipurge as u = ipurge (ipurge as u) u"
+  proof -
+    have "\<forall>as u. ipurge as u = ipurge (ipurge as u) u"
+      proof -
+      {
+        fix as
+        have "\<forall>u. ipurge as u = ipurge (ipurge as u) u"
+          proof(induct as)
+            case Nil show ?case by simp
+          next
+            case (Cons b bs)
+            assume a0: "\<forall>u. ipurge bs u = ipurge (ipurge bs u) u"
+            show ?case
+            proof -
+            {
+              fix u
+              have "ipurge (b # bs) u = ipurge (ipurge (b # bs) u) u "
+                proof(cases "domain b\<in>sources (b#bs) u")
+                  assume b0: "domain b\<in>sources (b#bs) u"
+                  then have b1: "ipurge (b # bs) u = b # ipurge bs u" by simp
+                  then have b2: "ipurge (ipurge (b # bs) u) u = ipurge (b # ipurge bs u) u" by simp
+                  have b3: "sources (b#bs) u = sources (b#ipurge bs u) u" using sources_ipurge by (metis b1) 
+                  with b1 b2 show ?thesis using a0 by auto 
+                next
+                  assume b0: "\<not> domain b\<in>sources (b#bs) u"
+                  then have b1: "ipurge (b # bs) u = ipurge bs u" by simp
+                  then have b2: "ipurge (ipurge (b # bs) u) u = ipurge (ipurge bs u) u" by simp
+                  with b1 show ?thesis  using a0 by auto 
+                qed
+            }
+            then show ?thesis by auto
+            qed
+          qed
+      }
+      then show ?thesis by auto
+      qed
+    then show ?thesis by auto
+  qed
 
+definition exec_equiv :: "'s \<Rightarrow> 'a list \<Rightarrow> 'd \<Rightarrow> 's  \<Rightarrow> 'a list \<Rightarrow> bool" ("(_ \<lhd> _ \<simeq> _ \<simeq> _ \<lhd> _)" [80,80,80,80,80] 75)
+    where "exec_equiv S as u T bs \<equiv> \<forall>S' T'. ((S,S')\<in> run as \<and> (T,T')\<in> run bs) \<longrightarrow>  (S' \<guillemotright> u = T' \<guillemotright> u)"
+
+lemma exec_equiv_sym : "(S \<lhd> as \<simeq> u \<simeq> T \<lhd> bs) \<Longrightarrow> (T \<lhd> bs \<simeq> u \<simeq> S \<lhd> as)"
+  by (metis exec_equiv_def)
 
 lemma exec_equiv_both:
-   "\<lbrakk>reachable0 m s; reachable0 m t; \<forall>s' t'. (s, s') \<in> step m a \<and> (t, t') \<in> step m b
-    \<longrightarrow> exec_equiv m s' as t' bs u\<rbrakk> \<Longrightarrow> exec_equiv m s (a # as) t (b # bs) u"
+   "\<lbrakk>reachable0 s; reachable0 t; \<forall>s' t'. (s, s') \<in> step a \<and> (t, t') \<in> step b
+    \<longrightarrow>  s' \<lhd> as \<simeq> u \<simeq> t' \<lhd> bs\<rbrakk> \<Longrightarrow> s \<lhd> (a # as) \<simeq> u \<simeq> t \<lhd> (b # bs) "
 proof -
-  assume a0: "reachable0 m s"
-  assume a1: "reachable0 m t"
-  assume a2: "\<forall>s' t'. (s, s') \<in> step m a \<and> (t, t') \<in> step m b \<longrightarrow> exec_equiv m s' as t' bs u"
-  have "\<forall>s'' t''. (s, s'') \<in> run m (a # as) \<and> (t, t'') \<in> run m (b # bs) \<longrightarrow> obs m u s'' = obs m u t''"
+  assume a0: "reachable0  s"
+  assume a1: "reachable0  t"
+  assume a2: " \<forall>s' t'. (s, s') \<in> step a \<and> (t, t') \<in> step b\<longrightarrow>  s' \<lhd> as \<simeq> u \<simeq> t' \<lhd> bs"
+  have "\<forall>s'' t''. (s, s'') \<in> run (a # as) \<and> (t, t'') \<in> run (b # bs) \<longrightarrow> s'' \<guillemotright> u = t'' \<guillemotright> u"
   proof -
     {
       fix s'' t''
-      assume b0: "(s, s'') \<in> run m (a # as) \<and> (t, t'') \<in> run m (b # bs)"
-      then obtain s' where b1: " (s, s') \<in> step m a \<and> (s',s'') \<in> run m as"
+      assume b0: "(s, s'') \<in> run (a # as) \<and> (t, t'') \<in> run (b # bs)"
+      then obtain s' where b1: " (s, s') \<in> step a \<and> (s',s'') \<in> run as"
         by auto
-      from b0 obtain t' where b2: "(t, t') \<in> step m b \<and> (t', t'') \<in> run m bs"
+      from b0 obtain t' where b2: "(t, t') \<in> step b \<and> (t', t'') \<in> run bs"
         by auto
-      with a2 b1 have b3: "exec_equiv m s' as t' bs u" by blast
-      with b0 b1 b2 have "obs m u s'' = obs m u t''" using exec_equiv_def 
+      with a2 b1 have b3: "s' \<lhd> as \<simeq> u \<simeq> t' \<lhd> bs" by blast
+      with b0 b1 b2 have "s'' \<guillemotright> u = t'' \<guillemotright> u" using exec_equiv_def 
         by fastforce
     }
     then show ?thesis by auto
@@ -186,177 +270,39 @@ proof -
     by metis
 qed
 
-lemma sources_ipurge: "sources m (ipurge m as u) u = sources m as u"
-proof -
-  have "\<forall>as u. sources m (ipurge m as u) u = sources m as u"
-  proof -
-    {
-      fix as
-      have "\<forall>u. sources m (ipurge m as u) u = sources m as u"
-      proof(induct as)
-        case Nil show ?case by simp
-      next
-        case (Cons b bs)
-        assume a0: "\<forall>u. sources m (ipurge m bs u) u = sources m bs u"
-        show ?case
-        proof -
-          {
-            fix u
-            have "sources m (ipurge m (b # bs) u) u = sources m (b # bs) u"
-            proof(cases "(domain m) b \<in> sources m (b#bs) u")
-              assume b0: "(domain m) b \<in> sources m (b#bs) u"
-              then have b1: "ipurge m (b # bs) u = b # ipurge m bs u"
-                by (simp add: sources_Cons) 
-              from a0 have b2: "sources m (ipurge m bs u) u = sources m bs u" by simp
-              from b1 have b3: "sources m (ipurge m (b # bs) u) u = sources m (b # ipurge m bs u) u" by simp
-              then have b40: "sources m (ipurge m (b # bs) u) u = sources m (ipurge m bs u) u \<union> 
-                         {w. w = (domain m) b \<and> (\<exists>v. interference m w v \<and> v \<in> sources m bs u)}"
-                by (simp add: b2 sources_Cons)
-              with b0 b2 have b41: "(domain m) b \<in> sources m (ipurge m (b # bs) u) u"
-                by (metis sources_Cons)
-              then have  b4: "sources m (ipurge m (b # bs) u) u = {(domain m) b} \<union> sources m (ipurge m bs u) u"
-                using b40 by auto
-              from b0 have b5: "sources m (b # bs) u = {(domain m) b} \<union> sources m bs u"
-                using sources_Cons by fastforce
-              then show ?thesis using a0 b4 by auto 
-            next
-              assume b0: "\<not> domain m b \<in> sources m (b#bs) u"
-              then have b1: "sources m (ipurge m (b # bs) u) u = sources m (ipurge m bs u) u" 
-                using sources_Cons by auto 
-              from b0 have b2: "sources m (b # bs) u = sources m bs u" 
-                by (smt (verit) Collect_empty_eq UnI2 mem_Collect_eq sources_Cons sup_bot_left sup_commute)
-              with a0 b1 show ?thesis by auto
-            qed
-          }
-          then show ?thesis by auto
-        qed
-      qed
-    }
-    then show ?thesis by auto
-  qed
-  then show ?thesis by auto
-qed
-
-lemma ipurge_eq: "ipurge m as u = ipurge m (ipurge m as u) u"
-proof -
-  have "\<forall>as u. ipurge m as u = ipurge m (ipurge m as u) u"
-  proof -
-    {
-      fix as
-      have "\<forall>u. ipurge m as u = ipurge m (ipurge m as u) u"
-      proof(induct as)
-        case Nil show ?case by simp
-      next
-        case (Cons b bs)
-        assume a0: "\<forall>u. ipurge m bs u = ipurge m (ipurge m bs u) u"
-        show ?case
-        proof -
-          {
-            fix u
-            have "ipurge m (b # bs) u = ipurge m (ipurge m (b # bs) u) u "
-            proof(cases "(domain m) b \<in> sources m (b#bs) u")
-              assume b0: "(domain m) b\<in> sources m (b#bs) u"
-              then have b1: "ipurge m (b # bs) u = b # ipurge m bs u" by simp
-              then have b2: "ipurge m (ipurge m (b # bs) u) u = ipurge m (b # ipurge m bs u) u" by simp
-              have b3: "sources m (b#bs) u = sources m (b#ipurge m bs u) u" using sources_ipurge by (metis b1)
-              with b1 b2 show ?thesis using a0 by auto 
-            next
-              assume b0: "\<not> (domain m) b\<in> sources m (b#bs) u"
-              then have b1: "ipurge m (b # bs) u = ipurge m bs u" by simp
-              then have b2: "ipurge m (ipurge m (b # bs) u) u = ipurge m (ipurge m bs u) u" by simp
-              with b1 show ?thesis  using a0 by auto 
-            qed
-          }
-          then show ?thesis by auto
-        qed
-      qed
-    }
-    then show ?thesis by auto
-  qed
-  then show ?thesis by auto
-qed
-
-
-
 (* Rushby's noninterference*)
-definition noninterference0 :: "('s, 'd, 'a, 'o) SM \<Rightarrow> bool"
-  where "noninterference0 m \<equiv> \<forall>u as. exec_equiv m (s0 m) as (s0 m) (ipurge m as u) u"
+definition noninterference0 :: "bool"
+  where "noninterference0 \<equiv> \<forall>u as. (s0 \<lhd> as \<simeq> u \<simeq> s0 \<lhd> (ipurge as u))"
 
 (* reachable state version of Rushby's noninterference*)
-definition noninterference0_r :: "('s, 'd, 'a, 'o) SM \<Rightarrow> bool"
-  where "noninterference0_r m \<equiv> \<forall>u as s. reachable0 m s \<longrightarrow> exec_equiv m s as s (ipurge m as u) u"
+definition noninterference0_r :: "bool"
+  where "noninterference0_r \<equiv> \<forall>u as s. reachable0 s \<longrightarrow> (s \<lhd> as \<simeq> u \<simeq> s \<lhd> (ipurge as u))"
 
 (* Oheimb's nondeterministic version of noninterference *)
 (* It is the same as Oheimb's strong noninterference*)
-definition noninterference1 :: "('s, 'd, 'a, 'o) SM \<Rightarrow> bool" 
-  where "noninterference1 m \<equiv> \<forall>u as bs. (ipurge m as u = ipurge m bs u) \<longrightarrow> 
-         exec_equiv m (s0 m) as (s0 m) bs u"
+definition noninterference1 :: "bool" where
+  "noninterference1 \<equiv> \<forall>u as bs. (ipurge as u = ipurge bs u)  \<longrightarrow> (s0 \<lhd> as \<simeq> u \<simeq> s0 \<lhd> bs)"
 
 (* reachable state version of Oheimb's strong noninterference *)
-definition noninterference1_r :: "('s, 'd, 'a, 'o) SM \<Rightarrow> bool"
-  where "noninterference1_r m \<equiv> \<forall>u as bs s. reachable0 m s \<longrightarrow> ipurge m as u = ipurge m bs u 
-         \<longrightarrow> exec_equiv m s as s bs u"
+definition noninterference1_r :: "bool"
+      where "noninterference1_r \<equiv> \<forall>u as bs s. reachable0 s \<longrightarrow> ipurge as u = ipurge bs u \<longrightarrow> (s \<lhd> as \<simeq> u \<simeq> s \<lhd> bs)"
 
 (* Oheimb's nonleakage. The Murray's nonleakage is the same *)
-definition nonleakage :: "('s, 'd, 'a, 'o) SM \<Rightarrow> bool" where
-  "nonleakage m \<equiv> \<forall>as s t u. (reachable0 m s) \<and> (reachable0 m t) \<longrightarrow> ivpeq m s (sources m as u) t  
-                                 \<longrightarrow> exec_equiv m s as t as u"
+definition nonleakage :: "bool" where
+  "nonleakage \<equiv> \<forall>as s t u. (reachable0 s) \<and> (reachable0 t) \<longrightarrow> (s \<approx>(sources as u)\<approx> t) 
+                                 \<longrightarrow> (s \<lhd> as \<simeq> u \<simeq> t \<lhd> as)"
 
 (* Oheimb's noninfluence *)
-definition noninfluence0 ::"('s, 'd, 'a, 'o) SM \<Rightarrow> bool" where
-  "noninfluence0 m \<equiv> \<forall> u as s t . (reachable0 m s) \<and> (reachable0 m t) \<longrightarrow> ivpeq m s (sources m as u) t 
-                                \<longrightarrow> exec_equiv m s as t (ipurge m as u) u"
+definition noninfluence0 ::"bool" where
+  "noninfluence0 \<equiv> \<forall> u as s t . (reachable0 s) \<and> (reachable0 t) \<longrightarrow> (s \<approx>(sources as u)\<approx> t) 
+                                \<longrightarrow> (s \<lhd> as \<simeq> u \<simeq> t \<lhd> (ipurge as u))"
 
 (* Murray's noninfluence (without the scheduler) *)
 (* replacing ``ipurge bs {C1} u'' by ``ipurge bs {C2} u'' yields and equivalent property as stated in Murray's paper*)
-definition noninfluence1 :: "('s, 'd, 'a, 'o) SM \<Rightarrow> bool" where
-  "noninfluence1 m \<equiv> \<forall>as bs s t u. (reachable0 m s) \<and> (reachable0 m t) \<longrightarrow> ivpeq m s (sources m as u) t
-                     \<longrightarrow> ipurge m as u = ipurge m bs u \<longrightarrow> exec_equiv m s as t bs u"
+definition noninfluence1 :: "bool" where
+  "noninfluence1 \<equiv> \<forall>as bs s t u. (reachable0 s) \<and> (reachable0 t) \<longrightarrow> (s \<approx>(sources as u)\<approx> t)
+                                 \<longrightarrow> ipurge as u = ipurge bs u \<longrightarrow> (s \<lhd> as \<simeq> u \<simeq> t \<lhd> bs)"
 
-subsection \<open> Unwinding conditions and unwinding theorem \<close>
-
-definition observed_consistent :: "('s, 'd, 'a, 'o) SM \<Rightarrow> bool" where
- "observed_consistent m \<equiv> (\<forall> s t u. (vpeq m s u t) \<longrightarrow> obs m u s = obs m u t)"
-
-
-definition weak_step_consistent :: "('s, 'd, 'a, 'o) SM \<Rightarrow> bool" 
-  where "weak_step_consistent m \<equiv> \<forall>a d s t. reachable0 m s \<and> reachable0 m t \<longrightarrow> (vpeq m s d t) 
-                              \<and> ((interference m (domain m a) d) \<longrightarrow> vpeq m s ((domain m) a) t)
-                              \<longrightarrow> (\<forall> s' t'. (s,s') \<in> step m a \<and> (t,t') \<in> step m a 
-                              \<longrightarrow> vpeq m s' d t')"
-
-definition weak_step_consistent_e :: "('s, 'd, 'a, 'o) SM \<Rightarrow> 'a \<Rightarrow> bool"
-  where  "weak_step_consistent_e m a \<equiv> \<forall>d s t. reachable0 m s \<and> reachable0 m t \<longrightarrow> (vpeq m s d t) 
-                              \<and> ((interference m (domain m a) d) \<longrightarrow> vpeq m s (domain m a) t)
-                              \<longrightarrow> (\<forall> s' t'. (s,s') \<in> step m a \<and> (t,t') \<in> step m a 
-                              \<longrightarrow> vpeq m s' d t')"
-
-    
-definition local_respect :: "('s, 'd, 'a, 'o) SM  \<Rightarrow> bool" 
-  where "local_respect m \<equiv> \<forall> a d s s'. reachable0 m s \<longrightarrow> (\<not> interference m ((domain m) a) d) 
-                          \<and> (s,s') \<in> step m a \<longrightarrow> (vpeq m s d s')"
-
-definition local_respect_e :: "('s, 'd, 'a, 'o) SM  \<Rightarrow> 'a \<Rightarrow> bool" 
-  where  "local_respect_e m a \<equiv> \<forall> d s s'. reachable0 m s \<longrightarrow> (\<not> (interference m) ((domain m) a) d) 
-                          \<and> (s,s') \<in> step m a \<longrightarrow> (vpeq m s d s')"
-
-lemma local_respect_all_evt : "local_respect m = (\<forall>a. local_respect_e m a)"
-  by (simp add: local_respect_def local_respect_e_def)
-
-lemma weak_step_consistent_all_evt : "weak_step_consistent m = (\<forall>a. weak_step_consistent_e m a)"
-  by (simp add:weak_step_consistent_def weak_step_consistent_e_def)
-
-locale SM_IFS = 
-  fixes m :: "('s, 'd, 'a, 'o) SM"
-  assumes 
-    vpeq_transitive_lemma : "\<forall>s t r d. vpeq m s d t \<and> vpeq m t d r \<longrightarrow> vpeq m s d r" and
-    vpeq_symmetric_lemma : "\<forall>s t d. vpeq m s d t \<longrightarrow> vpeq m t d s" and
-    vpeq_reflexive_lemma : "\<forall>s d. vpeq m s d s" 
-
-begin
-
-lemma exec_equiv_sym: "exec_equiv m s as t bs d \<Longrightarrow> exec_equiv m t bs s as d"
-  using exec_equiv_def vpeq_symmetric_lemma by metis
 
 subsection \<open>A Infererence Framework of Information Flow Security Properties\<close>
 (*
@@ -379,11 +325,11 @@ subsection \<open>A Infererence Framework of Information Flow Security Propertie
 
 *)
 
-lemma lm1: "noninterference0_r m \<Longrightarrow> noninterference0 m"
-  by (simp add: noninterference0_def noninterference0_r_def reachable_s0)
+lemma lm1: "noninterference0_r \<Longrightarrow> noninterference0"
+  using noninterference0_def noninterference0_r_def reachableC0 by blast
 
-lemma lm2: "noninterference1_r m \<Longrightarrow> noninterference1 m"
-  by (simp add: noninterference1_def noninterference1_r_def reachable_s0)
+lemma lm2: "noninterference1_r \<Longrightarrow> noninterference1"
+  using noninterference1_def noninterference1_r_def reachableC0 by blast
 
 (*
 lemma lm3: "noninterference0 \<Longrightarrow> noninterference1" sorry (*exec_equiv is not transitive, so this is not satisfied*)
@@ -392,58 +338,85 @@ lemma lm3: "noninterference0 \<Longrightarrow> noninterference1" sorry (*exec_eq
 lemma lm4: "noninterference0_r \<Longrightarrow> noninterference1_r" sorry (*exec_equiv is not transitive, so this is not satisfied*)
 *)
 
-lemma lm5: "noninfluence1 m \<Longrightarrow> nonleakage m" 
-  by (simp add: noninfluence1_def nonleakage_def)
+lemma lm5: "noninfluence1 \<Longrightarrow> nonleakage" 
+  using noninfluence1_def nonleakage_def by blast
 
 (*lemma lm11: "noninfluence0 \<Longrightarrow> nonleakage" *)
 
-lemma lm6: "noninfluence1 m \<Longrightarrow> noninterference1_r m" 
-  by (simp add: ivpeq_def noninfluence1_def noninterference1_r_def vpeq_reflexive_lemma)
+lemma lm6: "noninfluence1 \<Longrightarrow> noninterference1_r" 
+  using ivpeq_def noninfluence1_def noninterference1_r_def vpeq_reflexive by blast
 
-lemma lm7: "noninfluence0 m \<Longrightarrow> noninterference0_r m"
-  by (simp add: ivpeq_def noninfluence0_def noninterference0_r_def vpeq_reflexive_lemma)
+lemma lm7: "noninfluence0 \<Longrightarrow> noninterference0_r"
+  by (simp add: ivpeq_def noninfluence0_def noninterference0_r_def vpeq_reflexive)
 
-lemma lm8: "noninfluence1 m \<Longrightarrow> noninfluence0 m"
-  using ipurge_eq noninfluence0_def noninfluence1_def by fastforce
+lemma lm8: "noninfluence1 \<Longrightarrow> noninfluence0"
+  using ipurge_eq noninfluence0_def noninfluence1_def by blast 
   
-lemma lm9: "noninterference1_r m \<Longrightarrow> noninterference0_r m"
-  using ipurge_eq noninterference0_r_def noninterference1_r_def by fastforce
+lemma lm9: "noninterference1_r \<Longrightarrow> noninterference0_r"
+  using ipurge_eq noninterference0_r_def noninterference1_r_def by blast
 
-lemma lm10: "noninterference1 m \<Longrightarrow> noninterference0 m"
-  using ipurge_eq noninterference0_def noninterference1_def by fastforce
+lemma lm10: "noninterference1 \<Longrightarrow> noninterference0"
+  using ipurge_eq noninterference0_def noninterference1_def by blast
 
-subsection \<open>Unwinding Conditions\<close>
+subsection \<open> Unwinding conditions and unwinding theorem \<close>
+
+definition observed_consistent :: " bool" where
+ "observed_consistent \<equiv> \<forall>s t u. s \<sim>u\<sim> t \<longrightarrow> s \<guillemotright> u = t \<guillemotright> u"
+
+definition weak_step_consistent :: " bool" 
+  where "weak_step_consistent \<equiv> \<forall>a d s t. reachable0 s \<and> reachable0 t \<longrightarrow> s \<sim>d\<sim> t 
+                                \<and> (domain a \<leadsto> d \<longrightarrow> s \<sim>domain a\<sim> t) \<longrightarrow> (\<forall>s' t'. (s, s') \<in> step a 
+                                \<and> (t, t') \<in> step a \<longrightarrow> s' \<sim>d\<sim> t')"
+
+definition weak_step_consistent_e :: "'a \<Rightarrow> bool"
+  where  "weak_step_consistent_e a \<equiv> \<forall>d s t. reachable0 s \<and> reachable0 t \<longrightarrow> s \<sim>d\<sim> t 
+                                \<and> (domain a \<leadsto> d \<longrightarrow> s \<sim>domain a\<sim> t) \<longrightarrow> (\<forall>s' t'. (s, s') \<in> step a 
+                                \<and> (t, t') \<in> step a \<longrightarrow> s' \<sim>d\<sim> t')"
+
+    
+definition local_respect :: "bool" 
+  where "local_respect \<equiv> \<forall>a d s s'. reachable0 s \<longrightarrow> \<not> domain a \<leadsto> d \<and> (s, s') \<in> step a \<longrightarrow> s \<sim>d\<sim> s'"
+
+definition local_respect_e :: " 'a \<Rightarrow> bool" 
+  where  "local_respect_e a \<equiv> \<forall> d s s'. reachable0 s \<longrightarrow> \<not> domain a \<leadsto> d \<and> (s, s') \<in> step a \<longrightarrow> s \<sim>d\<sim> s'"
+
+lemma local_respect_all_evt : "local_respect = (\<forall>a. local_respect_e  a)"
+  by (simp add: local_respect_def local_respect_e_def)
+
+lemma weak_step_consistent_all_evt : "weak_step_consistent = (\<forall>a. weak_step_consistent_e a)"
+  by (simp add:weak_step_consistent_def weak_step_consistent_e_def)
+
 
 lemma sources_unwinding_step:
-    "\<lbrakk>ivpeq m s (sources m (a#as) d) t; weak_step_consistent m; (s, s') \<in> step m a; (t, t') \<in> step m a;
-      reachable0 m s; reachable0 m t\<rbrakk>  \<Longrightarrow> ivpeq m s' (sources m as d) t'"
+    "\<lbrakk>s \<approx> sources (a # as) d \<approx> t; weak_step_consistent; (s, s') \<in> step a; (t, t') \<in> step a;
+      reachable0  s; reachable0 t\<rbrakk>  \<Longrightarrow> s' \<approx> sources as d \<approx> t'"
 proof -
-  assume a0: "ivpeq m s (sources m (a#as) d) t"
-  assume a1: "weak_step_consistent m"
-  assume a2: "(s, s') \<in> step m a"
-  assume a3: "(t, t') \<in> step m a"
-  assume a4: "reachable0 m s"
-  assume a5: "reachable0 m t"
-  have a7: "sources m as d \<subseteq> sources m (a#as) d" by (simp add: sources_Cons) 
-  have "\<forall>u. u\<in> (sources m as d) \<longrightarrow> vpeq m s' u t'"
+  assume a0: "s \<approx> sources (a # as) d \<approx> t"
+  assume a1: "weak_step_consistent "
+  assume a2: "(s, s') \<in> step  a"
+  assume a3: "(t, t') \<in> step  a"
+  assume a4: "reachable0  s"
+  assume a5: "reachable0  t"
+  have a7: "sources  as d \<subseteq> sources  (a#as) d" by (simp add: sources_Cons) 
+  have "\<forall>u. u \<in> sources as d \<longrightarrow> s' \<sim>u\<sim> t'"
   proof -
     {
       fix u
-      assume b0: "u \<in> sources m as d"
-      from a7 b0 have b1: "u \<in> sources m (a#as) d" by auto
-      then have "vpeq m s' u t'"
-      proof(cases "interference m (domain m a) u")
-        assume c0: "interference m (domain m a) u"
+      assume b0: "u \<in> sources as d"
+      from a7 b0 have b1: "u \<in> sources (a#as) d" by auto
+      then have "s' \<sim>u\<sim> t'"
+      proof(cases "domain a \<leadsto> u")
+        assume c0: "domain a \<leadsto> u"
         show ?thesis
         proof -
-          have d0: "vpeq m s (domain m a) t"
+          have d0: "s \<sim>domain a\<sim> t"
             by (metis (mono_tags, lifting) CollectI UnI2 a0 b0 c0 ivpeq_def sources_Cons)
-          then have "vpeq m s' u t'" 
+          then have "s' \<sim>u\<sim> t'" 
             by (smt (verit, ccfv_SIG) a0 a1 a2 a3 a4 a5 b1 ivpeq_def weak_step_consistent_def)
           then show ?thesis by auto
         qed
       next
-        assume c0: "\<not> (interference m (domain m a) u)"
+        assume c0: "\<not> domain a \<leadsto> u"
         show ?thesis 
           by (smt (verit, best) a0 a1 a2 a3 a4 a5 b1 c0 ivpeq_def weak_step_consistent_def)
       qed
@@ -455,26 +428,26 @@ proof -
 qed
 
 lemma sources_preserved_left:
-  "\<lbrakk>local_respect m; reachable0 m s; reachable0 m t; (s, s') \<in> step m a; domain m a \<notin> sources m (a#as) u; 
-   ivpeq m s (sources m (a#as) u) t\<rbrakk> \<Longrightarrow> ivpeq m s' (sources m as u) t"
-  proof -
-    assume a1: "local_respect m"
-    assume a2: "reachable0 m s"
-    assume a3: "reachable0 m t"
-    assume a4: "(s, s') \<in> step m a"
-    assume a5: "domain m a \<notin> sources m (a#as) u"
-    assume a6: "ivpeq m s (sources m (a#as) u) t" 
-    have " \<forall>d\<in>sources m as u. vpeq m s' d t"
-    proof-
-      {
+  "\<lbrakk>local_respect; reachable0 s; reachable0 t; (s, s') \<in> step a; domain a \<notin> sources (a#as) u; 
+   s \<approx> sources (a # as) u \<approx> t\<rbrakk> \<Longrightarrow> s' \<approx> sources as u \<approx> t"
+proof -
+  assume a1: "local_respect"
+  assume a2: "reachable0 s"
+  assume a3: "reachable0 t"
+  assume a4: "(s, s') \<in> step a"
+  assume a5: "domain a \<notin> sources (a#as) u"
+  assume a6: "s \<approx> sources (a # as) u \<approx> t" 
+  have " \<forall>d\<in>sources as u. s' \<sim>d\<sim> t"
+  proof-
+    {
       fix d
-      assume b0: "d \<in> sources m as u"
-      then have b1: "\<not> interference m (domain m a) d" 
+      assume b0: "d \<in> sources as u"
+      then have b1: "\<not> domain a \<leadsto> d" 
         using a5 sources_Cons by fastforce
-      from a6 b0 have b2: "vpeq m s d t" 
+      from a6 b0 have b2: "s \<sim>d\<sim> t" 
         by (simp add: ivpeq_def sources_Cons)
-      with b1 have "vpeq m s' d t"
-        by (meson a1 a2 a4 local_respect_def vpeq_symmetric_lemma vpeq_transitive_lemma)
+      with b1 have "s' \<sim>d\<sim> t"
+        using a1 a2 a4 local_respect_def vpeq_symmetric vpeq_transitive by blast
     }
     then show ?thesis by simp
   qed
@@ -482,47 +455,45 @@ lemma sources_preserved_left:
 qed
 
 theorem UnwindingTheorem_nonleakage:
-    assumes p1: "observed_consistent m"
-    and     p2: "weak_step_consistent m"
-  shows "nonleakage m"
+    assumes p1: observed_consistent
+    and     p2: weak_step_consistent
+  shows nonleakage
 proof(subst nonleakage_def)
-  show "\<forall>as s t u. reachable0 m s \<and> reachable0 m t \<longrightarrow> ivpeq m s (sources m as u) t
-        \<longrightarrow> exec_equiv m s as t as u"
+  show "\<forall>as s t u. reachable0 s \<and> reachable0 t \<longrightarrow> (s \<approx>sources as u\<approx> t) \<longrightarrow> s \<lhd> as \<simeq> u \<simeq> t \<lhd> as"
   proof -
     {
       fix as
-      have "\<forall>s t u. reachable0 m s \<and> reachable0 m t \<longrightarrow> ivpeq m s (sources m as u) t
-           \<longrightarrow> exec_equiv m s as t as u"
+      have "\<forall>s t u. reachable0 s \<and> reachable0 t \<longrightarrow> (s \<approx>sources as u\<approx> t) \<longrightarrow> s \<lhd> as \<simeq> u \<simeq> t \<lhd> as"
       proof(induct as)
         case Nil
         show ?case 
         proof -
           {
             fix s t u
-            assume a0: "ivpeq m s (sources m [] u) t"
-            then have a1: "vpeq m s u t"
+            assume a0: "s \<approx>sources [] u\<approx> t"
+            then have a1: "s \<sim>u\<sim> t"
               by (simp add: ivpeq_def sources_Nil)
-            then have "exec_equiv m s [] t [] u"  unfolding exec_equiv_def
-              using observed_consistent_def p1 vpeq_def by fastforce
+            then have "s \<lhd> [] \<simeq> u \<simeq> t \<lhd> []"  unfolding exec_equiv_def
+              using observed_consistent_def p1 by auto
           }
           then show ?thesis by auto
         qed
       next
         case (Cons b bs)
-        assume a0: "\<forall>s t u. reachable0 m s \<and> reachable0 m t \<longrightarrow> ivpeq m s (sources m bs u) t
-                    \<longrightarrow> exec_equiv m s bs t bs u"
+        assume a0: "\<forall>s t u. reachable0 s \<and> reachable0 t \<longrightarrow> (s \<approx>sources bs u\<approx> t) \<longrightarrow> s \<lhd> bs \<simeq> u \<simeq> t \<lhd> bs"
         show ?case
         proof -
           {
             fix s t u
-            assume b0: "(reachable0 m s) \<and> (reachable0 m t)"
-            assume b1: "ivpeq m s (sources m (b#bs) u) t"
-            have "\<forall>s' t'. (s, s') \<in> step m b \<and> (t, t') \<in> step m b \<longrightarrow> exec_equiv m s' bs t' bs u"
-              by (meson a0 b0 b1 p2 reachableStep sources_unwinding_step)
-            then have "exec_equiv m s (b # bs) t  (b # bs) u" 
-              by (simp add: b0 exec_equiv_both)
+            assume b0: "(reachable0 s) \<and> (reachable0 t)"
+            assume b1: "s \<approx> sources (b # bs) u \<approx> t"
+            have "\<forall>s' t'. (s, s') \<in> step  b \<and> (t, t') \<in> step b \<longrightarrow> exec_equiv  s' bs u t' bs "
+              by (metis a0 b0 b1 p2 reachableStep sources_unwinding_step)
+            then have "s \<lhd> (b # bs) \<simeq> u \<simeq> t \<lhd> (b # bs) " 
+              using exec_equiv_def by auto
           }
-          then show ?thesis by auto
+          then show ?thesis
+            by blast
         qed
       qed
     }
@@ -530,63 +501,62 @@ proof(subst nonleakage_def)
   qed
 qed
 
+
 theorem UnwindingTheorem_noninfluence0:
-    assumes p1: "observed_consistent m" 
-    and     p2: "local_respect m"
-    and     p3: "weak_step_consistent m"
-  shows "noninfluence0 m"
+    assumes p1: observed_consistent 
+    and     p2: local_respect
+    and     p3: weak_step_consistent
+  shows noninfluence0
 proof(subst noninfluence0_def)
-  show "\<forall>u as s t. reachable0 m s \<and> reachable0 m t \<longrightarrow> ivpeq m s (sources m as u) t 
-        \<longrightarrow> exec_equiv m s as t (ipurge m as u) u"
+  show "\<forall>u as s t. reachable0 s \<and> reachable0 t \<longrightarrow> (s \<approx>sources as u\<approx> t) \<longrightarrow> s \<lhd> as \<simeq> u \<simeq> t \<lhd> ipurge as u"
   proof-
     {
       fix as
-      have "\<forall>u s t. reachable0 m s \<and> reachable0 m t \<longrightarrow> ivpeq m s (sources m as u) t 
-            \<longrightarrow> exec_equiv m s as t (ipurge m as u) u"
+      have "\<forall>u s t. reachable0 s \<and> reachable0 t \<longrightarrow> (s \<approx>sources as u\<approx> t) \<longrightarrow> s \<lhd> as \<simeq> u \<simeq> t \<lhd> ipurge as u"
       proof(induct as)
         case Nil show ?case 
         proof -
           {
             fix u s t
-            assume a0:"reachable0 m s \<and> reachable0 m t"
-            assume a1:"ivpeq m s (sources m [] u) t"
-            have a2:"vpeq m s u t" by (metis a1 insertI1 ivpeq_def sources_Nil)
-            have a3:"ipurge m [] u = []" by simp
-            from a2 have "exec_equiv m s [] t [] u" unfolding exec_equiv_def
-              using observed_consistent_def p1 vpeq_def by fastforce
-            with a3 have "exec_equiv m s [] t (ipurge m [] u) u" by auto
+            assume a0:"reachable0 s \<and> reachable0 t"
+            assume a1:" s \<approx> sources [] u \<approx> t"
+            have a2:" s \<sim>u\<sim> t" by (metis a1 insertI1 ivpeq_def sources_Nil)
+            have a3:"ipurge [] u = []" by simp
+            from a2 have "s \<lhd> [] \<simeq> u \<simeq> t \<lhd> []" unfolding exec_equiv_def
+              using observed_consistent_def p1 by auto
+            with a3 have " s \<lhd> [] \<simeq> u \<simeq> t \<lhd> ipurge [] u " by auto
           }
-          then show ?thesis by auto
+          then show ?thesis 
+            using UnwindingTheorem_nonleakage nonleakage_def p1 p3 by fastforce
         qed
       next
         case (Cons b bs)
-        assume a0:"\<forall>u s t. reachable0 m s \<and> reachable0 m t \<longrightarrow> ivpeq m s (sources m bs u) t 
-                   \<longrightarrow> exec_equiv m s bs t (ipurge m bs u) u"
+        assume a0:"\<forall>u s t. reachable0 s \<and> reachable0 t \<longrightarrow> (s \<approx>sources bs u\<approx> t) \<longrightarrow> s \<lhd> bs \<simeq> u \<simeq> t \<lhd> ipurge bs u"
         show ?case 
         proof-
           {
             fix u s t
-            assume b0:"reachable0 m s"
-            assume b1:"reachable0 m t"
-            assume b2:"ivpeq m s (sources m (b # bs) u) t"
-            have " exec_equiv m s (b # bs) t (ipurge m (b # bs) u) u"
-            proof(cases "domain m b \<in> sources m (b # bs) u")
-              assume d0: "domain m b \<in> sources m (b # bs) u"
-              then have d1: "ipurge m (b # bs) u = b # ipurge m bs u" by simp
-              have "\<forall>s' t'. (s, s') \<in> step m b \<and> (t, t') \<in> step m b \<longrightarrow> 
-                    exec_equiv m s' bs t' (ipurge m bs u) u"
+            assume b0:"reachable0 s"
+            assume b1:"reachable0 t"
+            assume b2:"s \<approx> sources (b # bs) u \<approx> t"
+            have " s \<lhd> (b # bs) \<simeq> u \<simeq> t \<lhd> ipurge (b # bs) u"
+            proof(cases "domain b \<in> sources (b # bs) u")
+              assume d0: "domain b \<in> sources (b # bs) u"
+              then have d1: "ipurge (b # bs) u = b # ipurge  bs u" by simp
+              then have " \<forall>s' t'. (s, s') \<in> step b \<and> (t, t') \<in> step b \<longrightarrow> s' \<lhd> bs \<simeq> u \<simeq> t' \<lhd> ipurge bs u"
                 by (meson a0 b0 b1 b2 p3 reachableStep sources_unwinding_step)
               then show ?thesis using b0 b1 d1 exec_equiv_both by auto
             next
-              assume d0: "\<not> domain m b \<in> sources m (b # bs) u"
-              then have d1: "ipurge m (b # bs) u = ipurge m bs u" by simp
-              have "\<forall>s'. (s, s') \<in> step m b \<longrightarrow> exec_equiv m s' bs t (ipurge m bs u) u"
+              assume d0: "\<not> domain b \<in> sources (b # bs) u"
+              then have d1: "ipurge (b # bs) u = ipurge bs u" by simp
+              have "\<forall>s'. (s, s') \<in> step  b \<longrightarrow> s' \<lhd> bs \<simeq> u \<simeq> t \<lhd> ipurge bs u"
                 by (meson a0 b0 b1 b2 d0 p2 reachableStep sources_preserved_left)
               then show ?thesis
                 by (smt (verit) d1 exec_equiv_def relcomp.cases run_Cons) 
             qed
           }
-          then show ?thesis by auto
+          then show ?thesis
+            by blast
         qed
       qed
     }
@@ -595,4 +565,5 @@ proof(subst noninfluence0_def)
 qed
 
 end
+
 end
